{
 "cells": [
  {
   "cell_type": "markdown",
   "metadata": {},
   "source": [
    "**ex 1.1**  \n",
    "Let $f:A \\longrightarrow B$ be any function with $U,V$ subset of $B$ and $X$ a subset of $A$.  Prove the following about the about the pre-image operation.  \n",
    "\n",
    "(**note:** $f^{-1}$ is the pre-image operation from the bottom of page 2 which is not a function and $f^{-1}$ *is not* the *function* $f^{-1}$ defined on a power set given on top of page 3 which is an unfortunate overloading of notation)  \n",
    "\n",
    "**also note:** $\\subset$ here should be interpreted as $\\subseteq$ **not** *as proper subset*  \n",
    "\n",
    "**(a)** $U\\subset V  \\implies f^{-1}(U) \\subset f^{-1}(V)$  \n",
    "note: ignoring the role of empty sets, this is pictorially obvious if we sketch out and shade circles for these sets \n",
    "\n",
    "(i) \n",
    "suppose $u \\in U$ has no preimage under $f$.  Then $f^{-1}(u) \\in f^{-1}(U)$ by construction \n",
    "and $f^{-1}(u) \\in f^{-1}(V)$ as this constains the empty set as well   \n",
    "*(note: treatment of empty sets should be cleaned up though this is worthwhile discussion point)*  \n",
    "\n",
    "(ii)  \n",
    "suppose $u \\in U$ has a preimage under $f$, then  \n",
    "$a = f^{-1}(u)$  \n",
    "and $f^{-1}(u) \\in f^{-1}(U)$ by construction and $f^{-1}(u)=a \\in f^{-1}(V)$  because $u\\in V$  \n",
    "\n",
    "**(b)** $f^{-1}(U\\cup V) = f^{-1}(U)\\cup f^{-1}( V)$  \n",
    "again this is pictorially obvious  \n",
    "for $u \\in U$  \n",
    "$f^{-1}(u) \\in f^{-1}(U\\cup V)$ by construction and   $f^{-1}(u) \\in f^{-1}(U)$ by construction  \n",
    "the argument is identical for $v$  \n",
    "\n",
    "\n",
    "**(c)** $f^{-1}(U\\cap V) = f^{-1}(U)\\cap f^{-1}( V)$  \n",
    "this is nearly implied by (a) since $U\\cap V \\subset U$ and $U\\cap V \\subset V$ then  \n",
    "$f^{-1}(U\\cap V)\\subset f^{-1}(U)\\cap  f^{-1}(V)$  \n",
    "a better approach is to use (b)  \n",
    "(i) supppose $U\\cap V = \\{\\}$  then  \n",
    "$f^{-1}(U\\cap V) = \\{\\}= f^{-1}(U)\\cap  f^{-1}(V)$   \n",
    "\n",
    "(ii) if they are not disjoint, then  biparition $U$ and $V$ such that $W := U \\cap V$  and $U= U' \\cup W$ (i.e. $U':=U-W$) and $V=V'\\cup W$ (i.e. $V':=V-W$) which implies $U' \\cap V' = \\{\\}$  \n",
    "\n",
    "Then  \n",
    "$f^{-1}\\big(U\\cap V\\big)$  \n",
    "$=f^{-1}\\big((U'\\cup W) \\cap (V'\\cup W)\\big)$  \n",
    "$=f^{-1}\\big((U'\\cap V') \\cup (U' \\cap W) \\cup (W\\cap V') \\cup (W\\cap W)\\big)$   \n",
    "$=f^{-1}\\big(\\{\\} \\cup \\{\\} \\cup \\{\\} \\cup W\\big)$   \n",
    "$=f^{-1}\\big(W\\big)$   \n",
    "$=f^{-1}\\big(W\\big)\\cap f^{-1}\\big(W\\big)$   \n",
    "$=\\Big(f^{-1}\\big(W\\big)\\cup f^{-1}\\big(U'\\big)\\Big)\\cap f^{-1}\\big(W\\big)$      \n",
    "$=\\Big(f^{-1}\\big(W\\big)\\cup f^{-1}\\big(U'\\big)\\Big)\\cap \\Big(f^{-1}\\big(W\\big)\\cup f^{-1}\\big(V'\\big)\\Big)$      \n",
    "$=f^{-1}\\big(W\\cup U'\\big)\\cap f^{-1}\\big(W\\cup V'\\big)$  (by b)      \n",
    "$=f^{-1}\\big(U)\\cap f^{-1}\\big(V\\big)$   \n",
    "\n",
    "**(d)** $f\\big(f^{-1}(U)\\big)\\subset U$   \n",
    "if $f^{-1}(U)=\\{\\}$, the result is immediate.  Otherwise write $U = U' \\cup U''$   \n",
    "where $U'$ contains all values with a non-empty pre-image under $f$ and $U'' = U-U'$.  Then    \n",
    "\n",
    "$f^{-1}(U)$  \n",
    "$=f^{-1}(U'\\cup U'')$  \n",
    "$=f^{-1}(U')\\cup f^{-1}(U'')$ (by b)   \n",
    "$=f^{-1}(U')\\cup \\{\\}$  \n",
    "$=f^{-1}(U')$   \n",
    "and  $f\\big(f^{-1}(U')\\big) =U$  (i.e. select arbitrary $u' \\in U'$ and for arbitrary $a\\in f^{-1}(u')$ we have $f(a) = u'$)  \\\n",
    "thus  \n",
    "$f\\big(f^{-1}(U)\\big)=f\\big(f^{-1}(U')\\big)= U'\\subset \\big(U'\\cup U''\\big) = U$   \n",
    "\n",
    "**(e)** for $X\\subset A$ then $X\\subset f^{-1}\\big(f(X)\\big)$  \n",
    "this is immediate: for $x\\in X$, $f(x) = y$ and then $y$ under the pre-image of $f$ by definition includes $x$.  Note this may be a proper subset.  In particular consider the restriction of $f$ to $X$ given by $f\\vert_{ X}$.  \n",
    "\n",
    "$X= f\\vert_{ X}^{-1}\\big(f\\vert_{ X}(X)\\big)$ and if $f$ is injective, then $f\\vert_{ X}^{-1}\\big(f\\vert_{ X}(X)\\big)=f^{-1}\\big(f(X)\\big)$  but if $f$ is not injective this need not be the case  \n",
    "\n",
    "\n",
    "**(f)** and **(g)** are if for any $U\\subset B$, $f\\big(f^{-1}(U)\\big)=U$ then $f$ is surjective and if for any $X\\subset A$, $f^{-1}\\big(f(X)\\big)=X$ then $f$ is injective, respectively.   \n",
    "\n",
    "\n",
    "note: the use of 'any' should be interpreted as 'arbitrary' i.e. in same manner as in analysis where we say \"for any $\\epsilon \\gt 0$ there exists $\\delta \\gt 0$...\"\n",
    "\n",
    "\n",
    "The results are nearly immediate: for the first case simply select $U:=B$ and by the argument in (d) this implies $U''$ has an empty pre-image under $f$ and hence it is empty thus $f$ is surjective.  The second case follows similarly, except let $X$ be a set containing an arbitrary single point $\\in A$, then $f^{-1}\\big(f(X)\\big)=X$ is the definition of injective-- i.e. every point in the image of $f$ has exactly one point in its pre-image (since the choice of point in $A$ was arbitrary).    \n"
   ]
  },
  {
   "cell_type": "markdown",
   "metadata": {},
   "source": [
    "**ex 1.3**  \n",
    "use Prop 1.8 (page 7)\n",
    "\n",
    "set $X:= \\mathbb Z$  \n",
    "\n",
    "$a := \\{0,1\\}$  \n",
    "$b := \\{-1,0\\}$  \n",
    "\n",
    "$a' := \\{1,2\\}$  \n",
    "$b' := \\{-1,-2\\}$  \n",
    "\n",
    "then  \n",
    "$\\mu(a,b) = \\{-1,0,1\\}$ and has cardinality 3  \n",
    "$\\mu(a',b') = \\{-2,-1,1,2\\}$ and has cardinality 4    \n",
    "$\\implies [\\mu(a,b)] \\neq [\\mu(a',b')]  $   \n",
    "hence our equivalence relation is not a congruence  "
   ]
  },
  {
   "cell_type": "code",
   "execution_count": null,
   "metadata": {},
   "outputs": [],
   "source": []
  },
  {
   "cell_type": "code",
   "execution_count": null,
   "metadata": {},
   "outputs": [],
   "source": []
  },
  {
   "cell_type": "code",
   "execution_count": null,
   "metadata": {},
   "outputs": [],
   "source": []
  }
 ],
 "metadata": {
  "kernelspec": {
   "display_name": "Python 3",
   "language": "python",
   "name": "python3"
  },
  "language_info": {
   "codemirror_mode": {
    "name": "ipython",
    "version": 3
   },
   "file_extension": ".py",
   "mimetype": "text/x-python",
   "name": "python",
   "nbconvert_exporter": "python",
   "pygments_lexer": "ipython3",
   "version": "3.8.5"
  }
 },
 "nbformat": 4,
 "nbformat_minor": 4
}
